src/proof/k8s_io/apimachinery/pkg/apis/meta/v1_init.v
@@ -1,5 +1,7 @@
 From New.proof Require Export prelude.
 From New.proof.k8s_io.apimachinery.pkg Require Export types_init.
+From New.proof.k8s_io.apimachinery.pkg.runtime Require Export schema_init.
+From New.proof.k8s_io.utils Require Export ptr_init.
 From New.proof Require Export time.
 Require Export New.generatedproof.k8s_io.apimachinery.pkg.apis.meta.v1.
 
